Vocab := Finset (Sum Nat Nat)
Note that both atomic propositions and atomic programs are `Nat``.
That is still the case now. But a `Vocab` now keeps track of
whether a `Nat`` was used as one or as the other kind of atom.

Previously a vocabulary was just a `Finset Nat` such that for example
the two PDL formulas `[1]2` and `[2]1` had the same vocabulary {1,2}
which affects the meaning of interpolation in a weird way.

Pdl/Fresh.lean
@@ -11,7 +11,7 @@ mutual
     | ⌈α⌉ φ => max (freshVarProg α) (freshVarForm φ)
   /-- Get a fresh atomic proposition `x` not occuring in `α`. -/
   def freshVarProg : Program → Nat
-    | ·c => c + 1
+    | ·c => 0 -- don't care!
     | α;'β  => max (freshVarProg α) (freshVarProg β)
     | α⋓β  =>  max (freshVarProg α) (freshVarProg β)
     | ∗α  => freshVarProg α
@@ -21,50 +21,58 @@ end
 open HasVocabulary
 
 mutual
-theorem freshVarForm_is_larger (φ) : ∀ n ∈ voc φ, n < freshVarForm φ := by
+theorem freshVarForm_is_larger (φ) : ∀ n ∈ (vocabOfFormula φ).atomProps, n < freshVarForm φ := by
   cases φ
-  all_goals simp [freshVarForm, voc, vocabOfFormula, not_or]
+  all_goals simp [freshVarForm, voc, vocabOfFormula, not_or, Vocab.atomProps]
   case neg φ =>
-    apply freshVarForm_is_larger
+    have IH := freshVarForm_is_larger φ
+    simp [Vocab.atomProps] at *
+    assumption
   case and φ1 φ2 =>
     have IH1 := freshVarForm_is_larger φ1
     have IH2 := freshVarForm_is_larger φ2
+    simp [Vocab.atomProps] at *
     aesop
   case box α φ =>
     have IHφ := freshVarForm_is_larger φ
     have IHα := freshVarProg_is_larger α
+    simp [Vocab.atomProps] at *
     aesop
 
-theorem freshVarProg_is_larger (α) : ∀ n ∈ voc α, n < freshVarProg α := by
+theorem freshVarProg_is_larger (α) : ∀ n ∈ (vocabOfProgram α).atomProps, n < freshVarProg α := by
   cases α
-  all_goals simp [freshVarProg, voc, vocabOfProgram]
+  all_goals simp [freshVarProg, voc, vocabOfProgram, Vocab.atomProps]
   case union α β =>
     have IHα := freshVarProg_is_larger α
     have IHβ := freshVarProg_is_larger β
+    simp [Vocab.atomProps] at *
     aesop
   case sequence α β =>
     have IHα := freshVarProg_is_larger α
     have IHβ := freshVarProg_is_larger β
+    simp [Vocab.atomProps] at *
     aesop
   case star α =>
     have IHα := freshVarProg_is_larger α
+    simp [Vocab.atomProps] at *
     aesop
   case test φ =>
     have IHφ := freshVarForm_is_larger φ
+    simp [Vocab.atomProps] at *
     aesop
 end
 
-theorem freshVarForm_is_fresh (φ) : freshVarForm φ ∉ voc φ := by
+theorem freshVarForm_is_fresh (φ) : Sum.inl (freshVarForm φ) ∉ voc φ := by
   have := freshVarForm_is_larger φ
-  simp [freshVarForm, voc, vocabOfFormula] at *
+  simp [freshVarForm, voc, vocabOfFormula, Vocab.atomProps] at *
   by_contra hyp
   specialize this (freshVarForm φ)
   have := Nat.lt_irrefl (freshVarForm φ)
   tauto
 
-theorem freshVarProg_is_fresh (α) : freshVarProg α ∉ HasVocabulary.voc α := by
+theorem freshVarProg_is_fresh (α) : Sum.inl (freshVarProg α) ∉ vocabOfProgram α := by
   have := freshVarProg_is_larger α
-  simp [freshVarProg, voc, vocabOfFormula] at *
+  simp [freshVarProg, voc, vocabOfFormula, Vocab.atomProps] at *
   by_contra hyp
   specialize this (freshVarProg α)
   have := Nat.lt_irrefl (freshVarProg α)
