Pdl/Vocab.lean
@@ -2,42 +2,71 @@ import Pdl.Syntax
 
 import Mathlib.Data.Finset.Basic
 import Mathlib.Data.Finset.Union
+import Mathlib.Data.Finset.Fold
+
+abbrev Vocab := Finset (Sum Nat Nat)
+
+def Vocab.atomProps : Vocab → Finset Nat :=
+  fun X => X.biUnion (fun x => match x with | Sum.inl n => {n} | Sum.inr _ => {} )
+
+def Vocab.atomProgs : Vocab → Finset Nat :=
+  fun X => X.biUnion (fun x => match x with | Sum.inl _ => {} | Sum.inr n => {n} )
 
 mutual
-  def vocabOfProgram : Program → Finset Nat
-    | ·c => {c}
+  def vocabOfProgram : Program → Vocab
+    | ·n => {.inr n}
     | α;'β => vocabOfProgram α ∪ vocabOfProgram β
     | α ⋓ β => vocabOfProgram α ∪ vocabOfProgram β
     | ∗α => vocabOfProgram α
     | ?' φ => vocabOfFormula φ
-  def vocabOfFormula : Formula → Finset Nat
+  def vocabOfFormula : Formula → Vocab
     | ⊥ => ∅
-    | ·c => {c}
+    | ·n => {.inl n}
     | ~φ => vocabOfFormula φ
     | φ⋀ψ => vocabOfFormula φ ∪ vocabOfFormula ψ
     | ⌈α⌉ φ => vocabOfProgram α ∪ vocabOfFormula φ
 end
 
-def vocabOfSetFormula : Finset Formula → Finset Nat
-  | X => X.biUnion vocabOfFormula
-
-def vocabOfListFormula : List Formula → Finset Nat
-  | X => (X.toFinset).biUnion vocabOfFormula
-
-def vocabOfListProgram : List Program → Finset Nat
-  | X => (X.toFinset).biUnion vocabOfProgram
-
-theorem inVocList : ℓ ∈ vocabOfListFormula L ↔ ∃φ ∈ L, ℓ ∈ vocabOfFormula φ := by
-  simp only [vocabOfListFormula, Finset.mem_biUnion, List.mem_toFinset]
-
 class HasVocabulary (α : Type) where
-  voc : α → Finset Nat
+  voc : α → Vocab
+
+open HasVocabulary
 
 instance formulaHasVocabulary : HasVocabulary Formula := ⟨vocabOfFormula⟩
+
 instance programHasVocabulary : HasVocabulary Program := ⟨vocabOfProgram⟩
-instance finsetFormulaHasVocabulary : HasVocabulary (Finset Formula) := ⟨vocabOfSetFormula⟩
-instance listFormulaHasVocabulary : HasVocabulary (List Formula) := ⟨vocabOfListFormula⟩
-instance listProgramHasVocabulary : HasVocabulary (List Program) := ⟨vocabOfListProgram⟩
+
+def Vocab.fromList : (L : List Vocab) → Vocab
+| [] => {}
+| (v::vs) => v ∪ Vocab.fromList vs
+
+instance [HasVocabulary α] : HasVocabulary (List α) :=
+  ⟨fun X => .fromList (X.map voc)⟩
+
+instance [HasVocabulary α] : HasVocabulary (Finset α) :=
+  ⟨fun X => (X.biUnion (fun f => {voc f})).fold (fun x y => x ∪ y) {} id⟩
+
+theorem Vocab.fromListFormula_map_iff n (L : List Formula): n ∈ Vocab.fromList (L.map vocabOfFormula) ↔ ∃ φ ∈ L, n ∈ vocabOfFormula φ := by
+  induction L
+  · simp [fromList]
+  case cons h t IH =>
+    simp only [fromList, Finset.mem_union, List.mem_cons, exists_eq_or_imp]
+    rw [← IH]
+
+theorem Vocab.fromListProgram_map_iff n (L : List Program): n ∈ Vocab.fromList (L.map vocabOfProgram) ↔ ∃ α ∈ L, n ∈ vocabOfProgram α := by
+  induction L
+  · simp [fromList]
+  case cons h t IH =>
+    simp only [fromList, Finset.mem_union, List.mem_cons, exists_eq_or_imp]
+    rw [← IH]
+
+theorem inVocList {α} [HasVocabulary α] n (L : List α): n ∈ voc L ↔ ∃ φ ∈ L, n ∈ voc φ := by
+  induction L
+  · simp [voc, Finset.mem_biUnion, List.mem_toFinset, Vocab.fromList]
+  case cons h t IH =>
+    simp only [voc, Vocab.fromList, Finset.mem_union, List.mem_cons, exists_eq_or_imp]
+    rw [← IH]
+    simp only [voc]
 
 /-- Test(α) -/
 def testsOfProgram : Program → List Formula
